added ord and ins function

Exercises3_1.thy
@@ -11,14 +11,78 @@ fun set :: "'a tree \<Rightarrow> 'a set" where
 "set Tip = {}" |
 "set (Node l a r) = {a} \<union> (set l) \<union> (set r)"
 
-value "(Suc 3) < (Suc 6)"
+(* find max among two int options *)
+fun max_opt :: "int option \<Rightarrow> int option \<Rightarrow> int option" where
+"max_opt None None = None" |
+"max_opt (Some a) None = Some a" |
+"max_opt None (Some b) = Some b" |
+"max_opt (Some a) (Some b) = Some(max a b)"
 
-fun ord_util :: "int tree \<Rightarrow> int \<Rightarrow> int"
+(* lemmas about max_opt*)
+lemma max_opt_COMMUTATIVE : "max_opt a b = max_opt b a"
+  apply(induction a; induction b)
+     apply(auto)
+  done
+
+lemma max_opt_ASSOCIATIVE : "max_opt (max_opt a b) c = max_opt a (max_opt b c)"
+  apply(induction a; induction b; induction c)
+         apply(auto)
+  done
+
+(* find min among two int options *)
+fun min_opt :: "int option \<Rightarrow> int option \<Rightarrow> int option" where
+"min_opt None None = None" |
+"min_opt (Some a) None = Some a" |
+"min_opt None (Some b) = Some b" |
+"min_opt (Some a) (Some b) = Some (min a b)"
+
+(* check if int option in lesser than int*)
+fun less_opt :: "int option \<Rightarrow> int \<Rightarrow> bool" where
+"less_opt None _ = True" |
+"less_opt (Some a) b = (a \<le> b)"
+
+(* check if int option is greater than int*)
+fun greater_opt :: "int option \<Rightarrow> int \<Rightarrow> bool" where
+"greater_opt None _ = True" |
+"greater_opt (Some a) b = (a \<ge> b)"
+
+(* find max element in subtree *)
+fun max_tree :: "int tree \<Rightarrow> int option" where
+"max_tree Tip = None" |
+"max_tree (Node l a r) = max_opt (Some a) (max_opt (max_tree l) (max_tree r))"
+
+(* find min element in subtree*)
+fun min_tree :: "int tree \<Rightarrow> int option" where
+"min_tree Tip = None" |
+"min_tree (Node l a r) = min_opt (Some a) (max_opt (min_tree l) (min_tree r))"
 
 (* check if tree is ordered *)
 fun ord :: "int tree \<Rightarrow> bool" where
 "ord Tip = True" |
-"ord (Node l a r) = "
+"ord (Node l a r) = ((less_opt (max_tree l) a) \<and> (greater_opt (min_tree r) a) \<and> (ord l) \<and> (ord r))"
+
+(* insert element in binary ordered tree
+NOTE: element is always inserted as a leaf*)
+fun ins :: "int \<Rightarrow> int tree \<Rightarrow> int tree" where
+"ins e Tip = (Node Tip e Tip)" |
+"ins e (Node l a r) = (if (a=e) then (Node l a r) else (if (e < a) then (Node (ins e l) a r) else (Node l a (ins e r))))"
+
+(* theorems for insertion correctness*)
+(* theorem 1: correct addition of element *)
+theorem insert_correctness : "set (ins x t) = {x} \<union> (set t)"
+  apply(induction t)
+   apply(auto)
+  done
+
+lemma max_insert : "max_tree (ins i t) = max_opt (Some i) (max_tree t)"
+  apply(induction t)
+  apply(auto)
+
+(* theorem 2: preservation of order*)
+theorem order_correctness : "ord t \<Longrightarrow> ord (ins i t)"
+  apply(induction t)
+   apply(auto)
+
 
 
 end
